feat: (1.1&1.2): WIP

Project 1/Ex1.dfy
@@ -29,7 +29,25 @@ function Serialize(a : aexpr) : seq<code>
 */
 function Deserialize(cs : seq<code>) : seq<aexpr> 
 {
-  
+	reconstruct(cs, [])
+}
+
+function reconstruct(cs : seq<code>, aes : seq<aexpr>) : seq<aexpr>
+	decreases cs, aes
+	requires forall k : int :: 0 <= k < cs.Length && cs[k].UnOpCode? 
+	 ==> aes.Length > 0 // TODO idk if this works or necessary TODO
+	requires forall k : int :: 0 <= k < cs.Length && cs[k].BinOpCode? 
+	 ==> aes.Length > 1 // TODO possibly not necessary
+{
+	if (cs == [])
+	then aes
+	else
+		match cs[0] {
+			case VarCode(s) => reconstruct(cs[1..], [Var(s)] + aes)
+			case ValCode(i) => reconstruct(cs[1..], [Val(i)] + aes)
+			case UnOpCode(op) => reconstruct(cs[1..], [UnOp(op, aes[0])] + aes[1..])
+			case BinOpCode(op) => reconstruct(cs[1..], [BinOp(op, aes[0], aes[1])] + aes[2..])
+		}
 }
 
 
@@ -39,9 +57,79 @@ function Deserialize(cs : seq<code>) : seq<aexpr>
 lemma DeserializeProperty(e : aexpr)
   ensures Deserialize(Serialize(e)) == [ e ]
 {
- 
+	calc {
+		Deserialize(Serialize(e));
+		== { deserializePropertyAux(e, [], []); }
+	}
 }
 
+lemma deserializePropertyAux(e : aexpr, cs : seq<code>, aes : seq<aexpr>)
+	ensures reconstruct(Serialize(e) + cs, ts) == reconstruct(cs, [e] + ts)
+	// ensures Deserialize(Serialize(e)+cs) == Deserialize(cs) + [e] // idk if this is preferable
+{
+	match e {
+		// base case??
+		case Var(s) => 
+		 calc {
+			reconstruct(Serialize(e) + cs, ts);
+			==
+			reconstruct(Serialize(Var(s)) + cs, ts); // by case
+			==
+			reconstruct([VarCode(s)] + cs, ts); // by def of Serialize
+			==
+			reconstruct(cs, [Var(s)] + ts); // by def of reconstruct
+			==
+			reconstruct(cs, [e] + ts); // by case
+		 }
+		case Val(i) =>
+		 calc {
+			reconstruct(Serialize(e) + cs, ts);
+			==
+			reconstruct(Serialize(Val(i)) + cs, ts); // by case
+			==
+			reconstruct([ValCode(i)] + cs, ts); // by def of Serialize
+			==
+			reconstruct(cs, [Val(i)] + ts); // by def of reconstruct
+			==
+			reconstruct(cs, [e] + ts); // by case
+		 }
+		// induction case
+		case UnOp(op, expr) =>
+		 // assert?
+		 calc {
+			reconstruct(Serialize(e) + cs, ts);
+			==
+			reconstruct(Serialize(UnOp(op, expr)) + cs, ts); // by case
+			==
+			reconstruct(Serialize(expr) + [UnOpCode(op)] + cs, ts); // def Serialize
+			== { deserializePropertyAux(expr, [UnOpCode(op)]+cs, ts); }
+			reconstruct([UnOpCode(op)] + cs, [expr] + ts); // IH
+			==
+			reconstruct(cs, [UnOp(op, expr)] + ts); // def reconstruct
+			==
+			reconstruct(cs, [e] + ts); // case
+		 }
+		case BinOp(op, expr1, expr2) =>
+		 assert [expr1] + ([expr2] + ts) == [expr1, expr2] + ts;
+		 calc {
+			reconstruct(Serialize(e) + cs, ts);
+			==
+			reconstruct(Serialize(BinOp(op, expr1, expr2)) + cs, ts); // by case
+			==
+			reconstruct(Serialize(expr2) + Serialize(expr1) + [BinOpCode(op)] + cs, ts); // def Serialize
+			== { deserializePropertyAux(expr2, (Serialize(expr1)+[BinOpCode(op)]+cs), ts); }
+			reconstruct(Serialize(expr1) + [BinOpCode(op)] + cs, [expr2] + ts); // IH
+			== { deserializePropertyAux(expr1, [BinOpCode(op)]+cs, [expr2] + ts); }
+			reconstruct([BinOpCode(op)] + cs, [expr1] + ([expr2] + ts)); // IH
+			==
+			reconstruct([BinOpCode(op)] + cs, [expr1, expr2] + ts); // properties of sequences
+			==
+			reconstruct(cs, [BinOp(op, expr1, expr2)] + ts); // def reconstruct
+			==
+			reconstruct(cs, [e] + ts); // case
+		 }
+	}
+}
 
 /*
   Ex1.3
